code/ecdsa/Hacl.Impl.EC.MontgomeryMultiplication.Lemmas.fst
@@ -27,7 +27,7 @@ open Hacl.Impl.EC.Setup
 
 #set-options "--z3rlimit 200"
 
-
+open Lib.Sequence
 
 val lemma_add_lt: a : int -> b: int -> q: int -> q1: int -> Lemma
   (requires (a < q /\ b < q1))
@@ -223,3 +223,313 @@ let lemma_multiplication_by_inverse_k0 #c a0 a_i a_i1 i =
 
   admit()
 
+
+
+
+
+
+val lemma_test: #l: size_nat -> c: curve ->  a: lseq uint64 l -> i: nat {i <= l} 
+  -> Lemma (ensures (
+    let a0 = sub a 0 i in 
+    let a1 = sub a i (l - i) in 
+    lseq_as_nat a = lseq_as_nat a0 + pow2 (64 * i) * lseq_as_nat a1))
+    (decreases (l - i))
+
+let rec lemma_test #l c a i = 
+  if i = 0 then begin 
+    let a0 = sub a 0 0 in 
+    let a1 = sub a 0 l in 
+    lseq_as_nat_last a0
+    end
+  else begin if i = l then lseq_as_nat_last (sub a l 0) else
+    begin 
+      let a0 = sub a 0 i in 
+      let a1 = sub a i (l - i) in 
+
+      calc (==) 
+      {
+  lseq_as_nat a1;
+  (==) {lemma_test #(l - i) c a1 1}
+  lseq_as_nat (sub a1 0 1) + pow2 64 * lseq_as_nat (sub a1 1 (l - i - 1));
+  (==) {lseq_as_nat_first (sub a1 0 1)}
+  v (index a1 0) + pow2 64 * lseq_as_nat (sub a1 1 (l - i - 1));
+  (==) {Seq.lemma_index_slice a 0 (i + 1) i}
+  v (index a i) + pow2 64 * lseq_as_nat (sub a (i + 1) (l - (i + 1)));
+      };
+    
+    assert(lseq_as_nat a1 - v (index a i) =  pow2 64 * lseq_as_nat (sub a (i + 1) (l - (i + 1))));
+
+    lemma_lseq_as_seq_extension (sub a 0 (i + 1)) (sub a 0 i) i;
+
+    let open FStar.Tactics in 
+    let open FStar.Tactics.Canon in 
+
+    
+    calc (==) {
+      lseq_as_nat a;
+      (==) {lemma_test c a (i + 1)}
+      lseq_as_nat (sub a 0 (i + 1)) + pow2 (64 * (i + 1)) * lseq_as_nat (sub a (i + 1) (l - (i + 1)));
+      (==) { pow2_plus (64 * i) 64}
+      lseq_as_nat (sub a 0 (i + 1)) + pow2 (64 * i) * pow2 64 * lseq_as_nat (sub a (i + 1) (l - (i + 1)));
+      (==) {assert_by_tactic (pow2 (64 * i) * pow2 64 * lseq_as_nat (sub a  (i + 1) (l - (i + 1))) == 
+  pow2 (64 * i) * (pow2 64 * lseq_as_nat (sub a (i + 1) (l - (i + 1))))) canon}
+      lseq_as_nat (sub a 0 (i + 1)) + pow2 (64 * i) * (pow2 64 * lseq_as_nat (sub a (i + 1) (l - (i + 1))));
+      (==) {assert(lseq_as_nat a1 - v (index a i) =  pow2 64 * lseq_as_nat (sub a (i + 1) (l - (i + 1))))}
+      lseq_as_nat (sub a 0 (i + 1)) - pow2 (64 * i) * v (index a i) + pow2 (64 * i) * lseq_as_nat a1; 
+      (==) {assert (lseq_as_nat (sub a 0 (i + 1)) == lseq_as_nat (sub a 0 i) + pow2 (64 * i) * v (index a i))}
+      lseq_as_nat (sub a 0 i) + pow2 (64 * i) * lseq_as_nat a1;}
+    end end
+
+
+
+open FStar.Math.Euclid 
+open FStar.Math.Fermat
+
+
+#push-options "--z3rlimit 100 --ifuel 0 --fuel 0"
+
+val lemma_division_is_multiplication:
+  t3: nat{t3 % pow2 64 = 0} ->
+  prime: pos {is_prime prime /\ prime > 3 /\ prime > pow2 64} -> 
+  Lemma (t3 * modp_inv2_prime (pow2 64) prime % prime = (t3 / pow2 64) % prime)
+
+let lemma_division_is_multiplication t3 prime =  
+
+  Hacl.Lemmas.P256.lemma_pow_mod_n_is_fpow prime (pow2 64 % prime) (prime - 2);
+  lemma_mod_twice (Spec.P256.pow (pow2 64 % prime) (prime - 2)) prime;
+
+  let open FStar.Tactics in 
+  let open FStar.Tactics.Canon in 
+
+  calc (==) {t3 * modp_inv2_prime (pow2 64) prime % prime;
+    (==) {FStar.Math.Lib.lemma_div_def t3 (pow2 64)}
+     pow2 64 * (t3 / pow2 64) * (Spec.P256.pow (pow2 64 % prime) (prime - 2) % prime) % prime;
+    (==) {assert_by_tactic (pow2 64 * (t3 / pow2 64) * (Spec.P256.pow (pow2 64 % prime) (prime - 2) % prime) % prime == 
+    (t3 / pow2 64) * (pow2 64 * (Spec.P256.pow (pow2 64 % prime) (prime - 2) % prime)) % prime) canon}
+    (t3 / pow2 64) * (pow2 64 * (Spec.P256.pow (pow2 64 % prime) (prime - 2) % prime)) % prime;
+    (==) {lemma_mod_mul_distr_r (t3 / pow2 64) (pow2 64 * (Spec.P256.pow (pow2 64 % prime) (prime - 2) % prime)) prime}
+    (t3 / pow2 64) * (pow2 64 * (Spec.P256.pow (pow2 64 % prime) (prime - 2) % prime) % prime) % prime;
+    (==) {Hacl.Lemmas.P256.power_distributivity (pow2 64) (prime - 2) prime}
+    (t3 / pow2 64) * (pow2 64 * (Spec.P256.pow (pow2 64) (prime - 2) % prime) % prime) % prime;
+    (==) {lemma_mod_mul_distr_r (pow2 64) (Spec.P256.pow (pow2 64) (prime - 2)) prime}
+    (t3 / pow2 64) * (pow2 64 * (Spec.P256.pow (pow2 64) (prime - 2)) % prime) % prime;
+    (==) {Hacl.Lemmas.P256.power_one_2 (pow2 64)}
+    (t3 / pow2 64) * (Spec.P256.pow (pow2 64) 1 * (Spec.P256.pow (pow2 64) (prime - 2)) % prime) % prime;
+    (==) {pow_plus (pow2 64) 1 (prime - 2)}
+    (t3 / pow2 64) * ((Spec.P256.pow (pow2 64) (prime - 1)) % prime) % prime;
+    (==) {  FStar.Math.Fermat.fermat_alt prime (pow2 64);
+      power_as_specification_same_as_fermat (pow2 64) (prime - 1)}
+    (t3 / pow2 64) % prime;
+  }
+
+
+
+
+
+val lemma_k0_computation: #c: curve-> t: nat -> k0 : uint64 {k0 == Hacl.Spec.Bignum.ModInv64.mod_inv_u64 (getLastWord #c)} ->
+  Lemma (let prime = getPrime c in  (t + prime * (((t % pow2 64) * v k0) % pow2 64)) % pow2 64 == 0)
+
+let lemma_k0_computation #c t k0 = 
+  let prime = getPrime c in 
+  let n0 = getLastWord #c in 
+
+  Hacl.Spec.Bignum.ModInv64.mod_inv_u64_lemma (getLastWord #c);
+
+  let k = t + prime * (((t % pow2 64) * v k0) % pow2 64) in  
+  lemma_mod_mul_distr_l t (v k0) (pow2 64);
+  lemma_mod_add_distr t (prime * (t * v k0 % pow2 64)) (pow2 64);
+  lemma_mod_mul_distr_r prime (t * v k0) (pow2 64);
+  
+  let open FStar.Tactics in 
+  let open FStar.Tactics.Canon in 
+
+
+  assert_by_tactic (prime * (t * v k0) == t * (prime * v k0)) canon;
+
+  assert(k % pow2 64 == (t + t * (prime * v k0) % pow2 64) % pow2 64);
+
+  lemma_mod_mul_distr_r t (prime * v k0) (pow2 64);
+  lemma_mod_mul_distr_l prime (v k0) (pow2 64);
+
+  assert(k % pow2 64 == (t + t * ((-1 + (1 + prime % pow2 64 * v k0)) % pow2 64) % pow2 64) % pow2 64);
+
+  lemma_mod_add_distr (-1) (1 + (prime) % pow2 64 * v k0) (pow2 64); 
+  lemma_mod_mul_distr_r t (-1) (pow2 64);
+  lemma_mod_add_distr t (t * (-1)) (pow2 64);
+  
+  assert(k % pow2 64 == 0)
+
+
+
+
+
+
+val montgomery_multiplication_one_round_proof: 
+  #c: curve ->
+  t: nat ->
+  k0 : uint64 {k0 == Hacl.Spec.Bignum.ModInv64.mod_inv_u64 (getLastWord #c)} ->
+  round: nat {round = (t + getPrime c * (((t % pow2 64) * v k0) % pow2 64)) / pow2 64} -> 
+  co: nat {co % getPrime c = t % getPrime c} -> 
+  Lemma (round  % getPrime c == co * (modp_inv2_prime (pow2 64) (getPrime c)) % ( getPrime c ))
+
+let montgomery_multiplication_one_round_proof #c t k0 round co =
+  let prime = getPrime c in 
+  let round = (t + prime * (((t % pow2 64) * v k0) % pow2 64)) / pow2 64 in 
+  assert(round % prime = (t + prime * (((t % pow2 64) * v k0) % pow2 64)) / pow2 64 % prime);
+
+  let k = t + prime * (((t % pow2 64) * v k0) % pow2 64) in 
+
+  lemma_k0_computation #c t k0;
+  assume (is_prime prime /\ prime > pow2 64);
+  lemma_division_is_multiplication k prime;
+
+  modulo_addition_lemma t prime (((t % pow2 64) * v k0) % pow2 64);
+
+  lemma_mod_mul_distr_l k (modp_inv2_prime (pow2 64) prime) prime;
+  lemma_mod_mul_distr_l co (modp_inv2_prime (pow2 64) prime) prime
+
+
+
+
+
+
+val lemma_up_bound0: #c: curve -> t0: nat {t0 < getPrime c * pow2 (64 * v (getCoordinateLenU64 c))} 
+  -> t: nat{let prime = getPrime c in t <= t0 / (pow2 (64 * v (getCoordinateLenU64 c))) + prime} -> 
+  Lemma (t < 2 * (getPrime c))
+
+let lemma_up_bound0 #c t0 t = 
+  let prime = getPrime c in 
+  let s = pow2 (64 * v (getCoordinateLenU64 c)) in 
+  lemma_mult_lt_left prime prime s;
+  assert(t0 < prime * s);
+  assert(t0 / s < prime);
+
+  assert(t < prime + prime)
+
+
+val lemma_up_bound1: #c: curve -> i: nat {i < v (getCoordinateLenU64 c)} 
+  -> t: nat {t < getPrime c * pow2 (64 * v (getCoordinateLenU64 c))}  
+  -> t0: nat {let prime = getPrime c in t0 <= t / (pow2 (64 * i)) + prime} 
+  -> k0: nat {k0 < pow2 64} 
+  -> t1: nat {t1 = (t0 + getPrime c * (((t0 % pow2 64) * k0) % pow2 64)) / pow2 64} -> 
+  Lemma (let prime = getPrime c in t1 <= t / (pow2 (64 * (i + 1))) + prime)
+
+let lemma_up_bound1 #c i t t0 k0 t1= 
+  let prime = getPrime c in 
+  assert(t0 <= t / (pow2 (64 * i)) + prime); 
+  assert(t1 = (t0 + prime * (((t0 % pow2 64) * k0) % pow2 64)) / pow2 64);
+  assert(((t0 % pow2 64) * k0) % pow2 64 <= pow2 64 - 1);
+  lemma_mult_le_left prime (((t0 % pow2 64) * k0) % pow2 64) (pow2 64 - 1);
+  assert(t1 <= (t0 + prime * (pow2 64 - 1)) / pow2 64);
+  assert(t1 <= (t0 + prime * pow2 64 - prime) / pow2 64); 
+  assert(t1 <= (t / (pow2 (64 * i)) / pow2 64 + prime));
+  division_multiplication_lemma t (pow2 (64 * i)) (pow2 64);
+  assert(t1 <= (t / (pow2 (64 * i) * pow2 64) + prime));
+  pow2_plus (64 * i) 64
+
+
+#push-options "--z3rlimit 100 --ifuel 2 --fuel 2"
+
+val lemma_mm_reduction: #c: curve -> a0: nat -> i: nat -> Lemma
+  (let prime = getPrime c in 
+    a0 * modp_inv2 #c (pow2 (i * 64)) * modp_inv2 #c (pow2 64) % prime == a0 * modp_inv2 #c (pow2 ((i + 1) * 64)) % prime)
+
+let lemma_mm_reduction #c a0 i = 
+  let open Spec.P256 in 
+  let prime = getPrime c in 
+  
+  let a = pow2 (i * 64) in 
+
+  let exp_prime: pos = prime - 2 in 
+
+  assert(modp_inv2 #c a == exp #prime (a % prime) exp_prime % prime);
+  Hacl.Lemmas.P256.lemma_pow_mod_n_is_fpow prime (a % prime) exp_prime;
+  lemma_mod_twice (pow (a % prime) exp_prime) prime;
+
+  assert(modp_inv2 #c (pow2 64) == exp #prime (pow2 64 % prime) exp_prime % prime);
+  Hacl.Lemmas.P256.lemma_pow_mod_n_is_fpow prime (pow2 64 % prime) exp_prime;
+  lemma_mod_twice (pow (pow2 64 % prime) exp_prime) prime;
+
+  Hacl.Lemmas.P256.power_distributivity_2 (a % prime) (pow2 64 % prime) exp_prime;
+
+
+  lemma_mod_mul_distr_r a0 (modp_inv2 #c a * modp_inv2 #c (pow2 64)) prime;
+
+  calc (==) {
+    modp_inv2 #c a * modp_inv2 #c (pow2 64) % prime;
+    (==) {}
+    (pow (a % prime) exp_prime % prime * (pow (pow2 64 % prime) exp_prime % prime)) % prime; 
+    (==) {lemma_mod_mul_distr_l (pow (a % prime) exp_prime) (pow (pow2 64 % prime) exp_prime % prime) prime}
+    (pow (a % prime) exp_prime * (pow (pow2 64 % prime) exp_prime % prime)) % prime; 
+    (==) {lemma_mod_mul_distr_r (pow (a % prime) exp_prime) (pow (pow2 64 % prime) exp_prime) prime}
+    (pow (a % prime) exp_prime * pow (pow2 64 % prime) exp_prime) % prime; 
+    (==) {pow_plus (a % prime) (pow2 64 % prime) exp_prime}
+    (pow (a % prime * (pow2 64 % prime)) exp_prime) % prime; 
+    (==) {Hacl.Lemmas.P256.power_distributivity (a % prime * (pow2 64 % prime)) exp_prime prime}
+    (pow (a % prime * (pow2 64 % prime) % prime) exp_prime) % prime; 
+    (==) {lemma_mod_mul_distr_l a (pow2 64 % prime) prime}
+    (pow ((a * (pow2 64 % prime)) % prime) exp_prime) % prime; 
+    (==) {lemma_mod_mul_distr_r a (pow2 64) prime}
+    (pow ((a * pow2 64) % prime) exp_prime) % prime; 
+    (==) {lemma_mod_twice (pow ((a * pow2 64) % prime) exp_prime) prime}
+    ((pow ((a * pow2 64) % prime) exp_prime) % prime) % prime; 
+    (==) {Hacl.Lemmas.P256.lemma_pow_mod_n_is_fpow prime (a * pow2 64 % prime) exp_prime} 
+    exp #prime ((a * pow2 64) % prime) exp_prime % prime; 
+    (==) {}
+    modp_inv2 #c (a * pow2 64);
+    (==) {pow2_plus (i * 64) 64}
+    modp_inv2 #c (pow2 ((i + 1) * 64));};
+
+  let open FStar.Tactics in 
+  let open FStar.Tactics.Canon in 
+
+  assert_by_tactic (a0 * modp_inv2 #c (pow2 (i * 64)) * modp_inv2 #c (pow2 64) % prime == a0 * (modp_inv2 #c (pow2 (i * 64)) * modp_inv2 #c (pow2 64)) % prime) canon
+
+#pop-options
+
+
+
+
+
+val lemma_mult_lt_center: a: nat -> b: nat -> c: pos -> d: pos -> Lemma
+    (requires (a < c /\ b < d))
+    (ensures (a * b < c * d))
+
+let lemma_mult_lt_center a b c d = ()
+
+
+val lemma_domain: #c: curve -> a: nat {a < getPrime c} -> b: nat {b < getPrime c} ->  k: nat ->
+  Lemma 
+    (requires (k == (a *  b * modp_inv2_prime (pow2 (getPower c)) (getPrime c)) % getPrime c))
+    (ensures (
+      k == toDomain_ #c (fromDomain_ #c a * fromDomain_ #c b % getPrime c) /\
+      k == toDomain_ #c (fromDomain_ #c a * fromDomain_ #c b)))
+
+let lemma_domain #c a b k = 
+  let prime = getPrime c in 
+  let multResult = a * b * modp_inv2_prime (pow2 (getPower c)) prime % prime in 
+
+  let mod = modp_inv2_prime (pow2 (getPower c)) prime in 
+  
+  calc (==) {
+    a * b * mod % prime;
+    (==) {lemmaFromDomainToDomain #c multResult}
+    toDomain_ #c (fromDomain_ #c multResult);
+    (==) {lemmaFromDomain #c multResult}
+    toDomain_ #c ((a * b * mod  % prime) * mod % prime);
+    (==) {lemma_mod_mul_distr_l (a * b * mod) mod prime}
+    toDomain_ #c (a * b * mod * mod % prime);
+    (==) {
+      let open FStar.Tactics in 
+      let open FStar.Tactics.Canon in 
+      assert_by_tactic (a * b * mod * mod == (a * mod) * (b * mod)) canon}
+    toDomain_ #c ((a * mod) * (b * mod) % prime);
+    (==) {
+      lemma_mod_mul_distr_l (a * mod) (b *  mod) prime; 
+      lemma_mod_mul_distr_r (a * mod % prime) (b * mod) prime}
+      
+    toDomain_ #c ((a * mod % prime) * (b * mod % prime) % prime);
+    (==) {lemmaFromDomain #c a; lemmaFromDomain #c b}
+    toDomain_ #c (fromDomain_ #c a * fromDomain_ #c b % prime);};
+
+    inDomain_mod_is_not_mod #c (fromDomain_ #c a * fromDomain_ #c b)
