code/ecdsa/Hacl.Impl.EC.P521.Reduction.fst
@@ -1,5 +1,50 @@
 module Hacl.Impl.EC.P521.Reduction
 
+open FStar.HyperStack.All
+open FStar.HyperStack
+module ST = FStar.HyperStack.ST
+
+open Lib.IntTypes 
+open FStar.Math.Lemmas
+open FStar.Math.Lib
+open Lib.Buffer
+
+open Hacl.SolinasReduction.Lemmas
+open Hacl.Impl.P256.LowLevel 
+
+open Spec.P256
+open Hacl.Spec.P256.Definition
+open FStar.Mul
+
+open Hacl.Impl.EC.MontgomeryMultiplication
+
+
+let coordinate521 = 9ul
+let prime521 = pow2 521 - 1
+
+assume val lemma_test: #l: size_nat -> c: curve ->  a: Lib.Sequence.lseq uint64 l -> i: nat {i <= l} -> 
+  Lemma (ensures (
+    let a0 = Lib.Sequence.sub a 0 i in 
+    let a1 = Lib.Sequence.sub a i (l - i) in 
+    lseq_as_nat a = lseq_as_nat a0 + pow2 (64 * i) * lseq_as_nat a1))
+    (decreases (l - i))
+
+
+val reduction_p521: i: lbuffer uint64 (coordinate521 *. 2ul) -> o: lbuffer uint64 coordinate521 -> 
+  Stack unit
+    (requires fun h -> live h i /\ live h o /\ disjoint i o /\ lseq_as_nat (as_seq h i) < prime521 * prime521)
+    (ensures fun h0 _ h1 -> modifies1 o h0 h1 /\ 
+      lseq_as_nat (as_seq h0 i) % prime521 == lseq_as_nat (as_seq h1 i))
+
+let reduction_p521 i o = 
+  let t0 = sub i (size 0) coordinate521 in 
+  let t1 = sub i coordinate521 coordinate521 in 
+
+  lemma_test 
+
+  admit()
+
+
 (* INPUT: An integer c = (c1041,..., c2, c1, c0) in base 2 with 0 ≤ c < p2
 521.
 OUTPUT: c mod p521.
